

# Variations on a linear parabolic PDE

Zoltan Leka

**Abstract.** The goal of this short note is to show how one linear parabolic PDE can be solved using three complementary methods: analytic, probabilistic, and spectral.

**Problem.** Let us consider the PDE

$$u_t = \frac{1}{2}u_{xx} - xu, -\infty < x < \infty \text{ and } t > 0$$

with the initial value condition  $u(x, 0) = f(x) \in L^1(\mathbb{R})$ . Find the general solution  $u$ .

**First solution.** To reduce the problem to the heat equation, we introduce the transformation

$$u(t, x) = e^{A(x,t)}v(x + B(t), t),$$

where  $v$  satisfies the heat equation  $v_t = \frac{1}{2}v_{xx}$  and  $v(x, 0) = f(x)$ . Straightforward computation shows that the PDE for  $u$  holds if and only if

$$A_t v + v_x B' + v_t = \frac{1}{2}A_{xx}v + \frac{1}{2}A_x^2 v + A_x v_x + \frac{1}{2}v_{xx} - xv.$$

Thus, from the equation  $B' = A_x$ , we obtain that  $A(x, t) = a(t)x + b(t)$ . Furthermore, from the equation  $A_t = \frac{1}{2}A_{xx} + \frac{1}{2}A_x^2 - x$ , we have  $a'(t)x + b'(t) = \frac{1}{2}a^2(t) - x$ . Hence,  $a'(t) = -1$  and  $a(t) = -t$ , and  $b(t) = t^3/6$  must hold. That is,  $A(x, t) = -xt + t^3/6$ . From  $B' = a(t)$ , we also have  $B(t) = -t^2/2$ . This implies

$$u(x, t) = e^{-xt+t^3/6}v(x - t^2/2, t).$$

From the heat kernel representation of  $v$ ,

$$u(x, t) = \frac{e^{-xt+t^3/6}}{\sqrt{2\pi t}} \int_{-\infty}^{\infty} f(s) e^{-\frac{(s-x+t^2/2)^2}{2t}} ds.$$

**Second solution.** This approach is based on the Feynman-Kac theory. The general solution to the diffusion equation is provided by

$$u(x, t) = \mathbb{E}\left(e^{-\int_0^t B_s ds} f(B_t) | B_0 = x\right),$$

where  $B_s$  is the Brownian motion. We now compute the expected value, which is a bit technical. Let us introduce the random variable

$$Y = \int_0^t B_s ds | B_0 = x.$$

From the tower property of the expectation,

$$u(x, t) = \mathbb{E}(\mathbb{E}(e^{-Y} f(B_t) | B_t = s)) = \int_{-\infty}^{\infty} \mathbb{E}(e^{-Y} | B_t = s) f(s) p_{B_t}(s) ds,$$

where  $p_{B_t}$  denotes the PDF of the variable  $B_t \sim N(x, t)$ .

Let us find the conditional expectation. It is simple to check that  $\mathbb{E}(Y) = \int_0^t x ds = tx$ , and

$$\mathbb{E}(Y^2) = \mathbb{E}\left(\int_0^t \int_0^t B_s B_r dr ds\right) = \int_0^t \int_0^t \mathbb{E}(B_s B_r) dr ds = \int_0^t \int_0^t \min(s, r) dr ds = \frac{t^3}{3}.$$

Similarly, we also obtain that

$$\mathbb{E}(Y B_t) = \int_0^t \mathbb{E}(B_s B_t) ds = \frac{t^2}{2}.$$

Hence,  $(B_t, Y)$  has a joint normal distribution

$$(B_t, Y) \sim N\left(\begin{bmatrix} x \\ xt \end{bmatrix}, \begin{bmatrix} t & t^2/2 \\ t^2/2 & t^3/3 \end{bmatrix}\right).$$

We recall that the conditional distribution of  $Y | B_t = s$  is normal with expectation  $t(x + s)/2$  and variance  $t^3/12$ . Thus, from the moment generating function of the normal variable,

$$\mathbb{E}(e^{-Y} | B_t = s) = e^{-t(x+s)/2 + t^3/24}.$$

We obtain

$$\int_{-\infty}^{\infty} \mathbb{E}(e^{-Y} | B_t = s) f(s) p_{B_t}(s) ds = \frac{1}{\sqrt{2\pi t}} \int_{-\infty}^{\infty} e^{-(x-s)^2/(2t)} e^{-t(x+s)/2 + t^3/24} f(s) ds.$$

Now, simple computation shows that the exponent can be written as a complete square, adding a few correction terms. Indeed,

$$\begin{aligned} -(x-s)^2/(2t) - t(x+s)/2 + t^3/24 \\ &= -(s-x+t^2/2)^2/(2t) + (x-t^2/2)^2/(2t) - x^2/(2t) - tx/2 + t^3/24 \\ &= -(s-x+t^2/2)^2/(2t) - tx + t^3/6. \end{aligned}$$

Thus,

$$u(x, t) = \frac{e^{-xt+t^3/6}}{\sqrt{2\pi t}} \int_{-\infty}^{\infty} f(s) e^{-\frac{(s-x+t^2/2)^2}{2t}} ds.$$

This expression coincides exactly with the result obtained via the gauge transformation method.

**Third solution.** We now apply Fourier theory to find the solution to the PDE. The Fourier transform of a function  $g \in L^1(\mathbb{R})$  is defined by

$$G(\omega) = \int_{-\infty}^{\infty} g(x) e^{-i\omega x} dx.$$

Let us take the Fourier transform of the PDE with respect to the spatial variable  $x$ . We obtain the first-order semilinear equation

$$U_t(\omega, t) + iU_\omega(\omega, t) = -\frac{\omega^2}{2}U(\omega, t) \text{ and } U(\omega, 0) = F(\omega).$$

We now solve the PDE by means of the method of characteristics. Formally, the system of characteristic ODEs is given by

$$\frac{dt}{1} = \frac{d\omega}{i} = \frac{dU}{-(\omega^2/2)U}.$$

Straightforward computation shows that

$$U(\omega, t) = e^{i\omega^3/6} F(\omega - it) e^{-i(\omega - it)^3/6}.$$

Hence,

$$U(\omega, t) = F(\omega - it) e^{t^3/6} e^{-(\omega - it)^2 t/2} e^{-i(\omega - it)t^2/2}.$$

Let us recall that how shift and exponential multiplication change the Fourier transform of an arbitrary function  $h$ :

$$h(x - a) \mapsto e^{-ia\omega} H(\omega) \quad \text{and} \quad e^{ax} h(x) \mapsto H(\omega + ia).$$

Moreover, the Fourier transform of the Gaussian distribution  $\frac{1}{\sqrt{2\pi t}} e^{-x^2/(2t)}$  is  $e^{-\omega^2 t/2}$ . Thus, the inverse Fourier of  $U$  is given by the rescaled convolution

$$u(x, t) = e^{t^3/6} e^{-xt} \left( \frac{1}{\sqrt{2\pi t}} e^{-(x-t^2/2)^2/(2t)} * f \right).$$

This representation agrees with the heat kernel expression derived in the previous two approaches, confirming the equivalence of the analytic, probabilistic, and spectral methods.